Avoid recent slowdown in MIPS proof.

compiler/targets/mips/mips_targetScript.sml
@@ -206,7 +206,14 @@ val mips_target_def = Define`
     ; proj := mips_proj
     |>`
 
-val (mips_config, mips_asm_ok) = asmLib.target_asm_rwts [] ``mips_config``
+val mips_reg_ok_def = Define`
+  mips_reg_ok n = ~MEM n mips_config.avoid_regs`
+
+val mips_reg_ok = save_thm("mips_reg_ok",
+  GSYM (SIMP_RULE (srw_ss()) [mips_config_def] mips_reg_ok_def))
+
+val (mips_config, mips_asm_ok) =
+  asmLib.target_asm_rwts [mips_reg_ok] ``mips_config``
 
 val mips_config = save_thm("mips_config", mips_config)
 val mips_asm_ok = save_thm("mips_asm_ok", mips_asm_ok)
